Finished the Bookstore with list implementation. Performance is underwhelming.

ADTExamples/QueryStructure/Bookstore.v
@@ -119,22 +119,380 @@ Definition Date := GetAttributeKey Orders "Date".
 
   Open Scope updateDef.
 
+  Require Import ProcessScheduler.AdditionalLemmas SetEq.
+
+  Lemma refine_SetEq_self {A} :
+    forall l : list A,
+      refine {l' | SetEq l' l}%comp
+             (ret l).
+  Proof.
+    unfold SetEq, refine; intros; inversion_by computes_to_inv.
+    econstructor; subst; split; eauto.
+  Qed.
+
+  Definition Equivalent_Ensembles {A : Type}
+             (P Q : Ensemble A) := forall a, P a <-> Q a.
+
+  Lemma Equivalent_In_EnsembleListEquivalence {A}
+        (qs : QueryStructureHint) (R : _)
+        (l : list _)
+        bod
+  : EnsembleListEquivalence (GetRelation qsHint R) l ->
+    Equivalent_Ensembles
+      (@Query_In qs A R bod)
+      (fun a => exists tup, List.In tup l /\ bod tup a).
+  Proof.
+    split; intros; unfold In in *.
+    destruct H0; eexists; intuition; eauto.
+    eapply H; eauto.
+    destruct H0; intuition; eexists; split; eauto.
+    eapply H; eauto.
+  Qed.
+
+  Definition Join_Lists {A B}
+             (l : list A)
+             (l' : list B)
+  : list (A * B) :=
+    fold_left (@app _) (map (fun a => map (fun b => (a, b)) l') l) nil.
+
+  Lemma In_fold_left_app {A}
+  : forall (l : list (list A))
+           (l'' : list A)
+           (a : A),
+      List.In a (fold_left (@app _) l l'') <->
+      (List.In a l'' \/ (exists l', List.In l' l /\ List.In a l')).
+  Proof.
+    induction l; simpl; intuition.
+    destruct_ex; intuition.
+    destruct (proj1 (IHl _ _) H).
+    apply in_app_or in H0; intuition; eauto.
+    destruct_ex; intuition; eauto.
+    eapply IHl; eauto using in_or_app.
+    destruct_ex; intuition; subst; eauto.
+    eapply IHl; eauto using in_or_app.
+    eapply IHl; eauto using in_or_app.
+  Qed.
+
+  Lemma In_Join_Lists {A B}
+  : forall (l : list A)
+           (l' : list B)
+           (a : A)
+           (b : B),
+      List.In (a, b) (Join_Lists l l') <->
+      (List.In a l /\ List.In b l').
+  Proof.
+    unfold Join_Lists; split; intros.
+    apply In_fold_left_app in H; simpl in *; intuition;
+    destruct_ex; intuition;
+    apply in_map_iff in H0; destruct_ex; intuition; subst;
+    apply in_map_iff in H1; destruct_ex; intuition; subst;
+    simpl; congruence.
+    intuition.
+    apply In_fold_left_app; right.
+    exists (map (fun b : B => (a, b)) l'); split;
+    apply in_map_iff; eexists; intuition; eauto.
+  Qed.
+
+  Lemma Equivalent_Join_Lists {A B}
+        (qs : QueryStructureHint) (R : _)
+        (l : list B)
+        (l' : list _)
+        bod
+  : EnsembleListEquivalence (GetRelation qsHint R) l' ->
+    Equivalent_Ensembles
+      (fun a => exists b, List.In b l /\
+                            (@Query_In qs A R (bod b) a))
+      (fun a => exists b, List.In b (Join_Lists l l') /\
+                          (bod (fst b) (snd b) a)).
+  Proof.
+    split; intros; unfold In in *.
+    - destruct H0; intuition; destruct H2; eexists; intuition; eauto.
+      unfold EnsembleListEquivalence in H.
+      apply In_Join_Lists; split; eauto.
+      eapply H; unfold In; apply H2.
+      simpl; auto.
+    - destruct_ex; intuition; destruct x; eexists; intuition.
+      eapply (In_Join_Lists l l'); eauto.
+      unfold Query_In; eexists; intuition; eauto.
+      apply H; eapply (In_Join_Lists l l'); eauto.
+  Qed.
+
+  Lemma Equivalent_List_In_Where {A B}
+        (l : list B)
+        (P : Ensemble B)
+        (bod : B -> Ensemble A)
+        (cond : B -> bool)
+        : (forall a, cond a = true <-> P a)
+          ->
+    Equivalent_Ensembles
+      (fun a : A => exists b, List.In b l /\ Query_Where (P b) (bod b) a)
+      (fun a : A => exists b, List.In b (filter cond l) /\ (bod b) a)
+  .
+  Proof.
+    split; intros; unfold In, Query_Where in *.
+    destruct H0; eexists; intuition; eauto.
+    eapply filter_In; split; eauto.
+    eapply H; eauto.
+    destruct H0; intuition; eexists; split; eauto.
+    eapply filter_In; eauto.
+    intuition; eauto using filter_In.
+    eapply H; eapply filter_In; eauto.
+  Qed.
+
+  Lemma Equivalent_Swap_In {A}
+        (qs : QueryStructureHint) (R R' : _)
+        (bod : Tuple -> Tuple -> Ensemble A)
+  :
+    Equivalent_Ensembles
+      (@Query_In qs _ R (fun tup => @Query_In qs _ R' (bod tup)))
+      (@Query_In qs _ R' (fun tup => @Query_In qs _ R
+                                               (fun tup' => bod tup' tup))).
+  Proof.
+    unfold Equivalent_Ensembles, Query_In; split; intros;
+    repeat (progress (destruct_ex; intuition)); eexists;
+    split; eauto.
+  Qed.
+
+  Lemma Equivalent_Swap_In_Where {A}
+        (qs : QueryStructureHint) (R : _)
+        {heading}
+        (bod : @Tuple heading -> Tuple -> Ensemble A)
+        (P : @Tuple heading -> Prop)
+  :
+    pointwise_relation
+      Tuple Equivalent_Ensembles
+      (fun tup' : Tuple =>
+         (@Query_In qs _ R
+                    (fun tup => Query_Where (P tup') (bod tup' tup))))
+      (fun tup' : Tuple =>
+         Query_Where (P tup') (@Query_In qs _ R (bod tup'))).
+  Proof.
+    unfold Equivalent_Ensembles, Query_In, Query_Where; split; intros;
+    repeat (progress (destruct_ex; intuition)); eexists;
+    split; eauto.
+  Qed.
+
+  Lemma refine_For_List_Return {A B}
+        (l : list B)
+        (extract : B -> A)
+  : refine
+      (For (fun a : A =>
+              exists b : B,
+                List.In b l /\ Return (extract b) a))%QuerySpec
+      (ret (map extract l)).
+  Proof.
+    unfold refine; intros; inversion_by computes_to_inv; subst.
+    econstructor; unfold In, Query_Return; split; intros.
+    eapply in_map_iff in H; destruct_ex; intuition; eauto.
+    eapply in_map_iff; destruct_ex; intuition; eauto.
+  Qed.
+
+  Add Parametric Morphism {A: Type} :
+    (Query_For)
+      with signature (@Equivalent_Ensembles A ==> refine)
+        as refine_Query_For_Equivalent.
+  Proof.
+    unfold impl, Query_For, refine; intros.
+    inversion_by computes_to_inv.
+    econstructor; split_iff; split; intros; eauto.
+    apply H; apply H1; auto.
+    apply H2; apply H; auto.
+  Qed.
+
+  Add Parametric Morphism {A: Type}
+      (qs : QueryStructureHint) (R : _)
+  :
+    (fun bod => Query_For (@Query_In qs _ R bod))
+      with signature ((pointwise_relation Tuple (@Equivalent_Ensembles A) ==> refine ))
+        as refine_Query_For_In_Equivalent.
+  Proof.
+    unfold impl, Query_For, pointwise_relation, Query_In, In, refine.
+    intros; inversion_by computes_to_inv.
+    econstructor; split_iff; split; intros; eauto.
+    destruct (H1 _ H0); eexists; intuition; eauto.
+    apply H; auto.
+    destruct_ex; apply H2; eexists; intuition; eauto.
+    apply H; auto.
+  Qed.
+
+  Lemma tupleAgree_refl :
+    forall (h : Heading)
+           (tup : @Tuple h)
+           (attrlist : list (Attributes h)),
+      tupleAgree tup tup attrlist.
+  Proof.
+    unfold tupleAgree; auto.
+  Qed.
+
+  Lemma refine_tupleAgree_refl_True :
+    forall (h : Heading)
+           (tup : @Tuple h)
+           (attrlist attrlist' : list (Attributes h)),
+      refine {b |
+              decides b (tupleAgree tup tup attrlist'
+                         -> tupleAgree tup tup attrlist)}
+             (ret true).
+  Proof.
+    unfold refine; intros; inversion_by computes_to_inv.
+    subst; econstructor; simpl; auto using tupleAgree_refl.
+  Qed.
+
+  Definition decideable_Heading_Domain
+             (h : Heading) :=
+    forall (idx : Attributes h)
+           (t t' : Domain h idx), {t = t'} + {t <> t'}.
+
+  Fixpoint Tuple_Agree_dec
+             (h : Heading)
+             (h_dec_eq : decideable_Heading_Domain h)
+             (attrlist : list (Attributes h))
+  : forall (tup tup' : Tuple),
+      {tupleAgree tup tup' attrlist} + {~tupleAgree tup tup' attrlist}.
+  Proof.
+  Admitted.
+
+  Lemma BookSchemaHeading_dec 
+    : decideable_Heading_Domain BookSchemaHeading.
+  Proof.
+  Admitted.
+
+  Fixpoint Check_List_Prop {A}
+           (cond : A -> bool)
+           (l : list A)
+  : bool :=
+    match l with
+        | [] => true
+        | a :: l' => if (cond a) then
+                          Check_List_Prop cond l'
+                        else false
+    end.
+
+  Definition In_List_Key 
+           (h : Heading)
+           (h_dec_eq : decideable_Heading_Domain h)
+           (attrlist : list (Attributes h))
+           (tup : Tuple)
+           (l : list Tuple) :=
+    Check_List_Prop (fun tup' => 
+                       if (Tuple_Agree_dec h_dec_eq attrlist tup tup')
+                       then true
+                       else false) l.
+
+  Lemma refine_unused_key_check
+  : forall (h : Heading)
+           (h_dec_eq : decideable_Heading_Domain h)
+           (attrlist attrlist' : list (Attributes h))
+           (tup : Tuple)
+           (rel : Ensemble Tuple)
+           (l : list Tuple),
+      EnsembleListEquivalence rel l
+      -> refine {b | decides b
+                             (forall tup' : Tuple,
+                                rel tup' ->
+                                tupleAgree tup tup' attrlist' ->
+                                tupleAgree tup tup' attrlist)}
+                (ret (In_List_Key h_dec_eq attrlist tup l)).
+  Admitted.
+
+  Lemma refine_unused_key_check'
+  : forall (h : Heading)
+           (h_dec_eq : decideable_Heading_Domain h)
+           (attrlist attrlist' : list (Attributes h))
+           (tup : Tuple)
+           (rel : Ensemble Tuple)
+           (l : list Tuple),
+      EnsembleListEquivalence rel l
+      -> refine {b | decides b
+                             (forall tup' : Tuple,
+                                rel tup' ->
+                                tupleAgree tup' tup attrlist' ->
+                                tupleAgree tup' tup attrlist)}
+                (ret (In_List_Key h_dec_eq attrlist tup l)).
+  Admitted.
+
+  Lemma refine_foreign_key_check 
+  : forall (h : Heading)
+           (rel : Ensemble Tuple)
+           (l : list Tuple)
+           (P : Ensemble Tuple)
+           (cond : Tuple -> bool),
+      EnsembleListEquivalence rel l
+      -> refine {b  |
+                 decides b
+                         (exists tup' : @Tuple h,
+                            rel tup' /\
+                            P tup')}
+                (ret (Check_List_Prop cond l)).
+    Admitted.
+
+  Lemma refine_pick_eq_ex_bind {A B : Type}
+        (P : A -> B -> Prop)
+        (a : A)
+  : refine (a' <- {a' | a' = a /\ exists b, P a' b};
+            {b | P a' b})
+           {b | P a b}.
+  Proof.
+    unfold refine; intros; inversion_by computes_to_inv;
+    econstructor; eauto.
+  Qed.
+
+  Lemma refine_under_if {A B} 
+        (P : A -> B -> Prop) : 
+    forall (cond : bool) (ta ea : A) ta' ea', 
+      refine {b | P ta b} ta'
+      -> refine {b | P ea b} ea'
+      -> refine {b | P (if cond then ta else ea) b}
+                (if cond then ta' else ea').
+  Proof.
+    intros; destruct cond; eauto.
+  Qed.
+
+  Lemma refine_if_ret {A}
+  : forall (cond : bool) (ta ea : A), 
+      refineEquiv (ret (if cond then ta else ea))
+                  (if cond then ret ta else ret ea).
+  Proof.
+    split; destruct cond; reflexivity.
+  Qed.
+
+  Definition BookStoreListImpl_SiR or (nr : (list Book) * (list Order)) : Prop :=
+    (EnsembleListEquivalence (GetUnConstrRelation or Books) (fst nr))
+    /\ (EnsembleListEquivalence (GetUnConstrRelation or Orders) (snd nr)).
+
   Definition BookStore :
     Sharpened BookStoreSpec.
   Proof.
     unfold BookStoreSpec.
+
+    hone representation' using (@DropQSConstraints_SiR _).
+
     (* Step 1: Decide what to do when inserting a book that
        violates the key constraints of Books. I think
        we will leave table unchanged when a 'bad' book is
        inserted. *)
     hone' mutator PlaceOrder.
     {
-      setoid_rewrite QSInsertSpec_refine with (default := ret r_n); simpl.
+      setoid_rewrite refineEquiv_pick_eq'.
+      simplify with monad laws.
+      apply refine_pick_forall_Prop with
+      (P := fun r_n or (n' : _) => _).
+      intros; setoid_rewrite QSInsertSpec_UnConstr_refine; simpl; eauto.
       setoid_rewrite decides_True.
       setoid_rewrite decides_3_True.
+      (* This takes 24 seconds on my machine.
+         The term size isn't the problem, as non of the goals
+         along the way are particularly large.
+
+         Time (setoid_rewrite refineEquiv_bind_unit;
+         setoid_rewrite refineEquiv_bind_unit;
+         setoid_rewrite refineEquiv_bind_unit;
+         setoid_rewrite refineEquiv_bind_unit) *)
       simplify with monad laws.
       unfold If_Then_Else; simpl.
       setoid_rewrite refine_if_bool_eta.
+      simplify with monad laws.
+      unfold SatisfiesSchemaConstraints; simpl; intros.
+      setoid_rewrite decides_2_True.
       simplify with monad laws.
       finish honing.
     }
@@ -142,23 +500,176 @@ Definition Date := GetAttributeKey Orders "Date".
        violates foreign key constraints of Orders. *)
     hone' mutator AddBook.
     {
-      setoid_rewrite QSInsertSpec_refine with (default := ret r_n); simpl.
+      setoid_rewrite refineEquiv_pick_eq'.
+      simplify with monad laws.
+      apply refine_pick_forall_Prop with
+      (P := fun r_n or (n' : _) => _).
+      intros; setoid_rewrite QSInsertSpec_UnConstr_refine; simpl; eauto.
       setoid_rewrite decides_True.
       setoid_rewrite decides_3_True.
       setoid_rewrite refineEquiv_bind_unit.
       unfold If_Then_Else; simpl.
       setoid_rewrite refine_if_bool_eta.
       simplify with monad laws.
-      remove_trivial_insertion_constraints r_n n Orders Books oISBN ISBN.
+      unfold SatisfiesSchemaConstraints; simpl; intros.
+      rewrite refine_tupleAgree_refl_True.
+      simplify with monad laws.
+      remove_trivial_insertion_constraints r_n n Orders Books oISBN ISBN H0.
       finish honing.
     }
 
-    (* Step 3: Hone representation to a list. Basically this should
-       amount to a bunch of refinements that show how to 'push' the
-       simulation relation through absmutator and absobserver by
-       providing implementations.
-       *)
+    hone representation' using BookStoreListImpl_SiR.
+
+    (* honing Get Titles. *)
+    hone' observer GetTitles using _.
+    { intros; subst.
+      set_evars; cbv delta [obsCod obsDom observerMethodType] beta in H; simpl in H.
+      apply refine_pick_forall_Prop with
+      (P := fun r_n or (n' : list string) => _).
+      intros; rewrite refine_pick_computes_to.
+      apply refine_pick_forall_Prop with
+      (P := fun r_n or (n' : list string) => _).
+      destruct H0; unfold DropQSConstraints_SiR; intros; subst.
+      intros; rewrite refine_pick_computes_to.
+      repeat rewrite GetRelDropConstraints in *.
+      setoid_rewrite Equivalent_In_EnsembleListEquivalence; simpl; eauto.
+      setoid_rewrite Equivalent_List_In_Where with
+      (cond := fun (a0 : Book) => if (string_dec (GetAttribute a0 Author) n) then true else false); simpl.
+      rewrite refine_For_List_Return.
+      unfold H; exact (reflexivity _).
+      intros; destruct (string_dec (a!Author)%Tuple n); split; intros;
+      auto; congruence.
+    }
+
+    (* honing Num Orders *)
+
+    hone' observer NumOrders using _.
+    {
+      intros; subst.
+      set_evars; cbv delta [obsCod obsDom observerMethodType] beta in H; simpl in H.
+      apply refine_pick_forall_Prop with
+      (P := fun r_n or (n' : _) => _).
+      intros; rewrite refine_pick_computes_to.
+      apply refine_pick_forall_Prop with
+      (P := fun r_n or (n' : _) => _).
+      unfold Count, DropQSConstraints_SiR; destruct H0; intros; subst.
+      repeat rewrite GetRelDropConstraints in *.
+      rewrite refine_pick_computes_to; eauto.
+      rewrite Equivalent_Swap_In.
+      rewrite refine_Query_For_In_Equivalent;
+        [ | apply Equivalent_Swap_In_Where with (qs := _)].
+      setoid_rewrite Equivalent_In_EnsembleListEquivalence; eauto.
+      setoid_rewrite Equivalent_List_In_Where with
+      (cond := fun a =>
+                 if (string_dec (a!Author)%Tuple n)
+                 then true
+                 else false); simpl.
+      setoid_rewrite Equivalent_Join_Lists; eauto.
+      setoid_rewrite Equivalent_List_In_Where with
+      (cond := fun ab =>
+               if (eq_nat_dec ((fst ab)!ISBN)%Tuple
+                              ((snd ab)!oISBN)%Tuple)
+               then true else false); simpl.
+    rewrite refine_For_List_Return.
+    simplify with monad laws.
+    unfold H; exact (reflexivity _).
+    { intros; destruct (eq_nat_dec ((fst a)!ISBN)%Tuple ((snd a)!oISBN)%Tuple);
+      split; intros; auto; congruence. }
+    { intros; destruct (string_dec (a!Author)%Tuple n); split; intros;
+    auto; congruence. }
+    }
+
+    hone' mutator AddBook.
+    {
+      setoid_rewrite refineEquiv_pick_eq'.
+      setoid_rewrite refineEquiv_unit_bind.
+      apply refine_pick_forall_Prop with
+      (P := fun r_n or (b : _)  => _).
+      setoid_rewrite refineEquiv_split_ex.
+      setoid_rewrite refineEquiv_pick_computes_to_and.
+      simplify with monad laws.
+      unfold SatisfiesSchemaConstraints; simpl; intros.
+      destruct H0.
+      setoid_rewrite refine_unused_key_check with 
+      (h_dec_eq := BookSchemaHeading_dec ); eauto.
+      simplify with monad laws. 
+      setoid_rewrite refine_unused_key_check' with
+      (h_dec_eq := BookSchemaHeading_dec ); eauto.
+      simplify with monad laws.
+      rewrite refine_pick_eq_ex_bind.
+      rewrite refine_under_if with (ea' := ret r_n); 
+        [ | reflexivity |
+          econstructor; inversion_by computes_to_inv; subst; 
+          constructor; eauto] .
+
+
+      Add Parametric Morphism {A: Type} (b : bool):
+        (If_Then_Else b)
+          with signature (
+            @refine A ==> @refine A ==> refine)
+            as refine_refine_if.
+      Proof.
+        unfold refine, If_Then_Else; intros.
+        destruct b; eauto.
+      Qed.
+
+      apply refine_refine_if; [ | reflexivity ].
+
+      apply refine_under_if with (ea' := ret r_n); 
+        [ | econstructor; inversion_by computes_to_inv; subst; 
+          constructor; eauto] .
+      unfold BookStoreListImpl_SiR; 
+        unfold GetUnConstrRelation, ith_Bounded; simpl.
+      erewrite refine_pick with (c := ret (n :: fst r_n, snd r_n)).
+      reflexivity.
+      intros x H3; apply computes_to_inv in H3; subst; eauto.
+      unfold GetUnConstrRelation, ith_Bounded,
+      EnsembleListEquivalence, RelationInsert, In in *; simpl in *;
+      split; intuition; eauto.
+      right; eapply H0; eauto.
+      right; eapply H0; eauto.
+    }
+
+    hone' mutator PlaceOrder.
+    {
+      setoid_rewrite refineEquiv_pick_eq'.
+      setoid_rewrite refineEquiv_unit_bind.
+      apply refine_pick_forall_Prop with
+      (P := fun r_n or (b : _)  => _).
+      setoid_rewrite refineEquiv_split_ex.
+      setoid_rewrite refineEquiv_pick_computes_to_and.
+      simplify with monad laws.
+      intros.
+      destruct H0; rewrite refine_foreign_key_check
+                   with (cond := fun a =>
+                                   if (eq_nat_dec (a!ISBN)%Tuple (n!oISBN)%Tuple)
+                                   then true
+                                   else false)
+
+; eauto.
+      simplify with monad laws.
+      rewrite refine_pick_eq_ex_bind.
+      rewrite refine_under_if with (ea' := ret r_n); 
+        [ | reflexivity |
+          econstructor; inversion_by computes_to_inv; subst; 
+          constructor; eauto] .
+      apply refine_refine_if; [ | reflexivity ].
+      unfold BookStoreListImpl_SiR; 
+        unfold GetUnConstrRelation, ith_Bounded; simpl.
+      erewrite refine_pick with (c := ret (fst r_n, n :: snd r_n)).
+      reflexivity.
+      intros x H3; apply computes_to_inv in H3; subst; eauto.
+      unfold GetUnConstrRelation, ith_Bounded,
+      EnsembleListEquivalence, RelationInsert, In in *; simpl in *;
+      split; intuition; eauto.
+      right; eapply H1; eauto.
+      right; eapply H1; eauto.
+    }      
+
     (* Step 4: Profit. :)*)
+
+    finish sharpening. 
+  Defined.
 
     (* Alternate 'simple' steps. *)
     (* Step 3: Add the '#Orders' attribute to Books schema. *)
@@ -174,9 +685,7 @@ Definition Date := GetAttributeKey Orders "Date".
     (* Step 4.1: Update mutators *)
     (* Step 4.2: Update observers *)
 
-  Admitted.
-
-  Definition BookStoreSchema' :=
+  (* Definition BookStoreSchema' :=
     query structure schema
       [ relation "Books" has
                 schema <"Author" : string,
@@ -187,7 +696,7 @@ Definition Date := GetAttributeKey Orders "Date".
         relation "Orders" has
                 schema <"ISBN" : nat,
                         "Date" : nat> ]
-      enforcing [attribute "ISBN" of "Orders" references "Books"].
+      enforcing [attribute "ISBN" of "Orders" references "Books"]. *)
 
   (*Definition AddAttribute_SiR
              (or : BookStoreRefRep)
